More work on the VDM model

theories/models/utp_vdm_simple/utp_vdm_expr.thy
@@ -1,11 +1,12 @@
 theory utp_vdm_expr
 imports 
+  "~~/src/HOL/Library/Option_ord"
   utp_vdm_sorts 
 begin
 
 default_sort vbasic
 
-typedef 'a vdme = "UNIV :: (vdmv WF_BINDING \<Rightarrow> 'a::vbasic) set" ..
+typedef 'a vdme = "UNIV :: (vdmv WF_BINDING \<rightharpoonup> 'a::vbasic) set" ..
 
 declare Rep_vdme [simp]
 declare Rep_vdme_inverse [simp]
@@ -19,6 +20,8 @@ lemma Rep_vdme_elim [elim]:
   "\<lbrakk> x = y; Rep_vdme x = Rep_vdme y \<Longrightarrow> P \<rbrakk> \<Longrightarrow> P"
   by (auto)
 
+setup_lifting type_definition_vdme
+
 notation Rep_vdme ("\<langle>_\<rangle>\<^sub>v")
 
 definition UNREST_VDME :: "(vdmv VAR) set \<Rightarrow> 'a vdme \<Rightarrow> bool" where
@@ -28,70 +31,76 @@ abbreviation MkVDVar :: "char list \<Rightarrow> 'a::vbasic itself \<Rightarrow>
 "MkVDVar n t \<equiv> (MkPlain n (embTYPE (Type t)) False)"
 
 definition VarE :: "string \<Rightarrow> 'a::vbasic vdme" ("$_") where
-"VarE n = Abs_vdme (\<lambda> b. the (Project (ProjBasicD (\<langle>b\<rangle>\<^sub>b (MkVDVar n TYPE('a))))))"
+"VarE n = Abs_vdme (\<lambda> b. Project (ProjBasicD (\<langle>b\<rangle>\<^sub>b (MkVDVar n TYPE('a)))))"
 
-lemma UNREST_VDME_VarE [unrest]: "UNREST_VDME (VAR - {MkVDVar n TYPE('a)}) ($n :: 'a vdme) "
+lemma UNREST_VDME_VarE [unrest]: "UNREST_VDME (VAR - {MkVDVar n TYPE('a)}) ($n :: 'a vdme)"
   by (simp add: UNREST_VDME_def VarE_def)
 
 declare [[coercion VarE]]
 
 definition LitE :: "'a::vbasic \<Rightarrow> 'a vdme" ("<_>") where
-"LitE x = Abs_vdme (\<lambda> b. x)"
+"LitE x = Abs_vdme (\<lambda> b. Some x)"
 
 lemma UNREST_VDME_LitE [unrest]: "UNREST_VDME vs <x>"
   by (simp add:UNREST_VDME_def LitE_def)
 
-definition UOpE :: "('a::vbasic \<Rightarrow> 'b::vbasic) \<Rightarrow> 'a vdme \<Rightarrow> 'b vdme" where
-"UOpE f v = Abs_vdme (\<lambda> b. f (Rep_vdme v b))"
+definition UOpE :: "('a::vbasic \<rightharpoonup> 'b::vbasic) \<Rightarrow> 'a vdme \<Rightarrow> 'b vdme" where
+"UOpE f v = Abs_vdme (\<lambda> b. (Rep_vdme v b) >>= f)"
+
+abbreviation UOpE' :: "('a::vbasic \<Rightarrow> 'b::vbasic)
+                      \<Rightarrow> 'a vdme \<Rightarrow> 'b vdme" where
+"UOpE' f \<equiv> UOpE (\<lambda> v. Some (f v))"
 
 lemma UNREST_VDME_UOpE [unrest]: "UNREST_VDME vs v \<Longrightarrow> UNREST_VDME vs (UOpE f v)"
   by (simp add:UNREST_VDME_def UOpE_def)
 
-definition BOpE :: "('a::vbasic \<Rightarrow> 'b::vbasic \<Rightarrow> 'c::vbasic) 
+definition BOpE :: "('a::vbasic \<rightharpoonup> 'b::vbasic \<rightharpoonup> 'c::vbasic) 
                    \<Rightarrow> 'a vdme \<Rightarrow> 'b vdme \<Rightarrow> 'c vdme" where
-"BOpE f v1 v2 = Abs_vdme (\<lambda> b. f (Rep_vdme v1 b) (Rep_vdme v2 b))"
+"BOpE f v1 v2 = Abs_vdme (\<lambda> b. do { x <- \<langle>v1\<rangle>\<^sub>v b; y <- \<langle>v2\<rangle>\<^sub>v b; g <- f x; g y })"
+
+abbreviation BOpE' :: "('a::vbasic \<Rightarrow> 'b::vbasic \<Rightarrow> 'c::vbasic)
+                      \<Rightarrow> 'a vdme \<Rightarrow> 'b vdme \<Rightarrow> 'c vdme" where
+"BOpE' f \<equiv> BOpE (\<lambda> v1. Some (\<lambda> v2. Some (f v1 v2)))"
 
 lemma UNREST_VDME_BOpE [unrest]: "\<lbrakk> UNREST_VDME vs v1; UNREST_VDME vs v2 \<rbrakk> \<Longrightarrow> UNREST_VDME vs (BOpE f v1 v2)"
   by (simp add:UNREST_VDME_def BOpE_def)
 
+fun sequence :: "'a option list \<Rightarrow> 'a list option" where
+"sequence [] = Some []" |
+"sequence (f # fs) = do { x \<leftarrow> f; xs \<leftarrow> sequence fs; Some (x # xs) }"
+
+abbreviation "mapM f \<equiv> sequence \<circ> map f"
+
+definition fset_option :: "'a option fset \<Rightarrow> 'a fset option" where
+"fset_option xs = (if (None \<in>\<^sub>f xs) then None else Some (the `\<^sub>f xs))"
+
+lemma fset_option_empty: 
+  "fset_option \<lbrace>\<rbrace> = Some \<lbrace>\<rbrace>"
+  by (simp add:fset_option_def)
+
 definition ListE :: "'a::vbasic vdme list \<Rightarrow> 'a list vdme" where
-"ListE xs = Abs_vdme (\<lambda> b. map (\<lambda> v. Rep_vdme v b) xs )"
+"ListE xs = Abs_vdme (\<lambda> b. mapM (\<lambda> v. \<langle>v\<rangle>\<^sub>v b) xs)"
 
 declare [[coercion ListE]]
 
-lemma UNREST_VDME_ListE [unrest]: "\<lbrakk> \<forall> x \<in> set xs. UNREST_VDME vs x \<rbrakk> \<Longrightarrow> UNREST_VDME vs (ListE xs)"
-  by (auto simp add:UNREST_VDME_def ListE_def)
+lemma UNREST_VDME_ListE [unrest]: 
+  "\<lbrakk> \<forall> x \<in> set xs. UNREST_VDME vs x \<rbrakk> \<Longrightarrow> UNREST_VDME vs (ListE xs)"
+  apply (induct xs)
+  apply (auto simp add:UNREST_VDME_def ListE_def)
+done
 
 definition FSetE :: "'a::vbasic vdme fset \<Rightarrow> 'a fset vdme" where
-"FSetE xs = Abs_vdme (\<lambda> b. (\<lambda> v. Rep_vdme v b) `\<^sub>f xs )"
+"FSetE xs = Abs_vdme (\<lambda> b. fset_option ((\<lambda> v. \<langle>v\<rangle>\<^sub>v b) `\<^sub>f xs))"
 
 declare [[coercion FSetE]]
 
-lemma UNREST_VDME_FSetE [unrest]: "\<lbrakk> \<forall> x \<in>\<^sub>f xs. UNREST_VDME vs x \<rbrakk> \<Longrightarrow> UNREST_VDME vs (FSetE xs)"
+lemma UNREST_VDME_FSetE [unrest]: 
+  "\<lbrakk> \<forall> x \<in>\<^sub>f xs. UNREST_VDME vs x \<rbrakk> \<Longrightarrow> UNREST_VDME vs (FSetE xs)"
   apply (simp add:UNREST_VDME_def FSetE_def)
   apply (clarify)
-  apply (simp add:fimage.rep_eq)
+  apply (simp add:fimage.rep_eq fset_option_def)
   apply (safe)
-  apply (metis imageI)+
-done
-
-definition SemE :: "'a::vbasic vdme \<Rightarrow> vdmv WF_EXPRESSION" where 
-"SemE f = Abs_WF_EXPRESSION (\<lambda> b. BasicD (Inject (Rep_vdme f b)))"
-
-lemma SemE_rep_eq: "\<langle>SemE f\<rangle>\<^sub>e = (\<lambda> b. BasicD (Inject (Rep_vdme f b)))"
-  apply (subgoal_tac "(\<lambda> b. BasicD (Inject (Rep_vdme f b))) \<in> WF_EXPRESSION")
-  apply (simp add:SemE_def)
-  apply (simp add:WF_EXPRESSION_def)
-  apply (rule_tac x="embTYPE (Type TYPE('a))" in exI)
-  apply (rule)
-  apply (simp add:type_rel_vdmt)
-  apply (metis Abs_UTYPE_inverse BasicD_type Defined_vdmv_def InjVB_def InjVB_nbot Inject_type embTYPE_def from_nat_to_nat prjTYPE_def vdmt_UTYPE)
-done
-
-lemma UNREST_EXPR_SemE [unrest]:
-  "UNREST_VDME vs e \<Longrightarrow> UNREST_EXPR vs (SemE e)"
-  by (simp add:UNREST_EXPR_def UNREST_VDME_def SemE_rep_eq)
-
+oops
 
 lemma embTYPE_inv_vdm [simp]: 
   "prjTYPE (embTYPE VTYPE('a) :: vdmv UTYPE) = VTYPE('a)"
@@ -101,34 +110,43 @@ lemma embTYPE_inv_vdm [simp]:
   apply (rule Inject_type)
 done
 
-(* Need this *)
+lift_definition SemE :: "'a::vbasic vdme \<Rightarrow> vdmv WF_EXPRESSION" is
+"\<lambda> f. (\<lambda> b. case \<langle>f\<rangle>\<^sub>v b of Some v \<Rightarrow> BasicD (Inject v) | None \<Rightarrow> \<bottom>\<^bsub>VTYPE('a)\<^esub>)"
+  apply (simp add:WF_EXPRESSION_def)
+  apply (rule_tac x="embTYPE VTYPE('a)" in exI)
+  apply (rule)
+  apply (simp add:type_rel_vdmt)
+  apply (case_tac "\<langle>vdme\<rangle>\<^sub>v b")
+  apply (auto)
+done
 
+lemma UNREST_EXPR_SemE [unrest]:
+  "UNREST_VDME vs e \<Longrightarrow> UNREST_EXPR vs (SemE e)"
+  by (simp add:UNREST_EXPR_def UNREST_VDME_def SemE.rep_eq)
 
 lemma SemE_expr_type [simp]: 
   "expr_type (SemE (v::'a vdme)) = embTYPE VTYPE('a)"
-  apply (simp add:expr_type_def etype_rel_def SemE_rep_eq type_rel_vdmt)
-  apply (rule the_equality)
+  apply (simp add:expr_type_def etype_rel_def SemE.rep_eq type_rel_vdmt)
+  apply (rule the_equality, rule)
+  apply (case_tac "\<langle>v\<rangle>\<^sub>v b")
   apply (auto)
+  apply (drule_tac x="\<B>" in spec)
+  apply (case_tac "\<langle>v\<rangle>\<^sub>v \<B>")
+  apply (auto)
+  apply (metis BasicD_type_cases BotI_type_cases prjTYPE_inv_vdm)
   apply (metis BasicD_type_cases Inject_type prjTYPE_inv_vdm vbasic_type_rel_uniq)
 done
 
-(*
-lemma SemE_type_string [simp]: "expr_type (SemE (v::string vdme)) = embTYPE StringT"
-  apply (simp)
-  apply (simp add:expr_type_def etype_rel_def SemE_rep_eq)
-  apply (rule the_equality)
-  apply (simp add:type_rel_vdmt)
-  apply (force simp add:Inject_list_def Inject_char_def)
-oops
+instantiation vdme :: (vbasic) DEFINED
+begin
 
+definition Defined_vdme :: "'a vdme \<Rightarrow> bool" where
+"\<D>(e) \<longleftrightarrow> (\<forall> b. (\<langle>e\<rangle>\<^sub>v b \<noteq> None))"
 
-lemma SemE_type: "expr_type (SemE (v::('a::vbasic) vdme)) = embTYPE (Type TYPE('a))"
-  apply (simp add:expr_type_def etype_rel_def SemE_rep_eq)
-  apply (rule the_equality)
-  apply (metis Abs_UTYPE_type BasicD_type Defined_vdmv_def InjVB_def InjVB_nbot Inject_type embTYPE_def utype_rel_vdmv_def)
-  apply (auto)
-oops
-*)
+instance ..
+
+end
+
 
 instantiation vdme :: ("{one,vbasic}") one
 begin
@@ -159,14 +177,14 @@ instance vdme :: ("{zero_neq_one,vbasic}") zero_neq_one
   apply (auto simp add:one_vdme_def zero_vdme_def LitE_def)
   apply (erule Rep_vdme_elim)
   apply (simp)
-  apply (metis zero_neq_one)
+  apply (metis option.inject zero_neq_one)
 done
   
 instantiation vdme :: ("{plus,vbasic}") plus
 begin
 
 definition plus_vdme :: "'a vdme \<Rightarrow> 'a vdme \<Rightarrow> 'a vdme" where
-"plus_vdme = BOpE (op +)"
+"plus_vdme = BOpE' (op +)"
 
 instance ..
 
@@ -180,7 +198,7 @@ instantiation vdme :: ("{minus,vbasic}") minus
 begin
 
 definition minus_vdme :: "'a vdme \<Rightarrow> 'a vdme \<Rightarrow> 'a vdme" where
-"minus_vdme = BOpE (op -)"
+"minus_vdme = BOpE' (op -)"
 
 instance ..
 
@@ -194,7 +212,7 @@ instantiation vdme :: ("{uminus,vbasic}") uminus
 begin
 
 definition uminus_vdme :: "'a vdme \<Rightarrow> 'a vdme" where
-"uminus_vdme = UOpE uminus"
+"uminus_vdme = UOpE' uminus"
 
 instance ..
 
@@ -208,7 +226,7 @@ instantiation vdme :: ("{times, vbasic}") times
 begin
 
 definition times_vdme :: "'a vdme \<Rightarrow> 'a vdme \<Rightarrow> 'a vdme" where
-"times_vdme = BOpE (op *)"
+"times_vdme = BOpE' (op *)"
 
 instance ..
 end
@@ -221,16 +239,16 @@ instantiation vdme :: ("{inverse,vbasic}") inverse
 begin
 
 definition inverse_vdme :: "'a vdme \<Rightarrow> 'a vdme" where
-"inverse_vdme = UOpE inverse"
+"inverse_vdme = UOpE' inverse"
 
 definition divide_vdme :: "'a vdme \<Rightarrow> 'a vdme \<Rightarrow> 'a vdme" where
-"divide_vdme = BOpE divide"
+"divide_vdme = BOpE' divide"
 
 instance ..
 
 end
 
-instantiation vdme :: ("{ord,vbasic}") ord
+instantiation vdme :: ("{preorder,vbasic}") ord
 begin
 
 definition less_eq_vdme :: "'a vdme \<Rightarrow> 'a vdme \<Rightarrow> bool" where
@@ -242,26 +260,24 @@ definition less_vdme :: "'a vdme \<Rightarrow> 'a vdme \<Rightarrow> bool" where
 instance ..
 end
 
-thm add_comm
-
-thm ab_semigroup_add.add_commute
-
 instance vdme :: ("{semigroup_add,vbasic}") semigroup_add
-  apply (intro_classes, auto simp add:plus_vdme_def BOpE_def add_assoc)
-  thm add_assoc
-  thm semigroup_add.add_assoc
-sorry
+  by (intro_classes, auto simp add:plus_vdme_def BOpE_def add_assoc)
 
 instance vdme :: ("{ab_semigroup_add,vbasic}") ab_semigroup_add
   apply (intro_classes)
-  apply (auto simp add:plus_vdme_def BOpE_def add_commute)
+  apply (auto simp add:plus_vdme_def BOpE_def)
+  apply (rule, rule ext, auto)
+  apply (case_tac "\<langle>a\<rangle>\<^sub>v x", auto, case_tac "\<langle>b\<rangle>\<^sub>v x", auto simp add:add_commute)
 done
 
 instance vdme :: ("{semigroup_mult, vbasic}") semigroup_mult
   by (intro_classes, auto simp add:times_vdme_def BOpE_def mult_assoc)
 
 instance vdme :: ("{ab_semigroup_mult,vbasic}") ab_semigroup_mult
-  by (intro_classes, auto simp add:times_vdme_def BOpE_def mult_commute)
+  apply (intro_classes, auto simp add:times_vdme_def BOpE_def)
+  apply (rule, rule ext, auto)
+  apply (case_tac "\<langle>a\<rangle>\<^sub>v x", auto, case_tac "\<langle>b\<rangle>\<^sub>v x", auto simp add:mult_commute)
+done
 
 (*
 instance vdme :: ("{comm_monoid_mult,vbasic}") comm_monoid_mult
@@ -269,16 +285,27 @@ instance vdme :: ("{comm_monoid_mult,vbasic}") comm_monoid_mult
 *)  
 
 instance vdme :: ("{semiring,vbasic}") semiring
-  by (intro_classes, auto simp add:plus_vdme_def times_vdme_def BOpE_def distrib_right distrib_left)
+  apply (intro_classes, auto simp add:plus_vdme_def times_vdme_def BOpE_def distrib_right distrib_left)
+  apply (rule, rule ext, auto)
+  apply (case_tac "\<langle>a\<rangle>\<^sub>v x", auto, case_tac "\<langle>b\<rangle>\<^sub>v x", auto, case_tac "\<langle>c\<rangle>\<^sub>v x", auto simp add:distrib_right)
+  apply (rule, rule ext, auto)
+  apply (case_tac "\<langle>a\<rangle>\<^sub>v x", auto)
+done
 
 instance vdme :: ("{comm_semiring,vbasic}") comm_semiring
-  by (intro_classes, auto simp add:plus_vdme_def times_vdme_def BOpE_def distrib)
+  apply (intro_classes, auto simp add:plus_vdme_def times_vdme_def BOpE_def distrib)
+  apply (rule, rule ext, auto)
+  apply (case_tac "\<langle>a\<rangle>\<^sub>v x", auto, case_tac "\<langle>b\<rangle>\<^sub>v x", auto, case_tac "\<langle>c\<rangle>\<^sub>v x", auto simp add:distrib)
+done
 
+(*
 instance vdme :: ("{semiring_0,vbasic}") semiring_0
-  by (intro_classes, auto simp add:plus_vdme_def times_vdme_def zero_vdme_def BOpE_def LitE_def ab_left_minus ab_diff_minus)
+  apply (intro_classes, auto simp add:plus_vdme_def times_vdme_def zero_vdme_def BOpE_def LitE_def ab_left_minus ab_diff_minus)
+  apply (rule, rule ext, auto, case_tac "\<langle>a\<rangle>\<^sub>v x", auto)
+
 
 instance vdme :: ("{semiring_1,vbasic}") semiring_1
-  by (intro_classes, auto simp add:times_vdme_def one_vdme_def BOpE_def LitE_def)
+  apply (intro_classes, auto simp add:times_vdme_def one_vdme_def BOpE_def LitE_def)
 
 instance vdme :: ("{ring,vbasic}") ring
   by (intro_classes, auto simp add:plus_vdme_def zero_vdme_def minus_vdme_def uminus_vdme_def BOpE_def UOpE_def LitE_def ab_left_minus ab_diff_minus)
@@ -288,19 +315,10 @@ instance vdme :: ("{ring_1,vbasic}") ring_1 ..
 instance vdme :: ("{comm_ring_1,vbasic}") comm_ring_1 
   by (intro_classes, auto simp add:times_vdme_def one_vdme_def BOpE_def LitE_def mult_1)
 
+
 instance vdme :: ("{numeral,vbasic}") numeral ..
-instance vdme :: ("{numeral,semiring_1,vbasic}") semiring_numeral ..
-
 (*
-abbreviation const_numerals :: "('a::{zero,ord,vbasic}) vdme set" where
-"const_numerals \<equiv> {0..}" 
-
-lemma "num_of_nat 4 = undefined"
-  apply (simp add:num_of_nat.simps)
-
-
-lemma "2 \<in> const_numerals"
-  apply (simp add: less_eq_vdme_def zero_vdme_def plus_vdme_def num_of_nat_def)
+instance vdme :: ("{numeral,semiring_1,vbasic}") semiring_numeral ..
 *)
 
 declare is_num_numeral [simp]
@@ -317,15 +335,16 @@ lemma UNREST_VDME_numeral [unrest]:
   apply (simp only:numeral_plus_numeral[symmetric] unrest)
   apply (simp only:numeral_plus_numeral[symmetric] numeral_One unrest)
 done
+*)
 
 definition dom :: "('a::{linorder,vbasic},'b::{linorder,vbasic}) fmap vdme \<Rightarrow> 'a fset vdme" where
-"dom \<equiv> UOpE fdom"
+"dom \<equiv> UOpE' fdom"
 
 definition ran :: "('a::{linorder,vbasic},'b::{linorder,vbasic}) fmap vdme \<Rightarrow> 'b fset vdme" where
-"ran \<equiv> UOpE fran"
+"ran \<equiv> UOpE' fran"
 
 definition card :: "('a::{linorder,vbasic}) fset vdme \<Rightarrow> nat vdme" where
-"card = UOpE fcard"
+"card = UOpE' fcard"
 
 syntax
   "_uexpr_vdme" :: "'a vdme \<Rightarrow> uexpr" ("_")
@@ -333,32 +352,33 @@ syntax
 translations
   "_uexpr_vdme e" == "CONST SemE e"
 
-lemma SemE_defined [defined]: "\<D> (SemE v)"
-  apply (simp add:Defined_WF_EXPRESSION_def SemE_rep_eq)
-  apply (metis Defined_vdmv_def InjVB_def InjVB_nbot)
+lemma SemE_defined [defined]: "\<D> v \<Longrightarrow> \<D> (SemE v)"
+  apply (auto simp add:Defined_WF_EXPRESSION_def Defined_vdme_def SemE.rep_eq)
+  apply (metis Defined_vdmv_def InjVB_def InjVB_nbot option.simps(5))
 done
 
 lemma SemE_type [typing]: 
   "SemE (v :: 'a vdme) :\<^sub>e embTYPE VTYPE('a)"
-  apply (simp add:etype_rel_def SemE_rep_eq)
-  apply (metis Abs_UTYPE_type BasicD_type Defined_vdmv_def InjVB_def InjVB_nbot Inject_type embTYPE_def utype_rel_vdmv_def)
+  apply (auto simp add:etype_rel_def SemE.rep_eq)
+  apply (case_tac "\<langle>v\<rangle>\<^sub>v b")
+  apply (auto simp add:type_rel_vdmt)
 done
 
 lemma SemE_EvalE_compat [typing]:
-  "vtype x = embTYPE VTYPE('a) \<Longrightarrow> \<lbrakk>SemE (v :: 'a vdme)\<rbrakk>\<epsilon>b \<rhd> x"
+  "\<lbrakk> \<D> v; vtype x = embTYPE VTYPE('a) \<rbrakk> \<Longrightarrow> \<lbrakk>SemE (v :: 'a vdme)\<rbrakk>\<epsilon>b \<rhd> x"
   apply (rule) back back
   apply (force intro:typing defined)
   apply (force intro:defined)
 done
 
 lemma SemE_expr_compat [typing]:
-  "vtype x = embTYPE VTYPE('a) \<Longrightarrow> SemE (v :: 'a vdme) \<rhd>\<^sub>e x"
+  "\<lbrakk> \<D> v; vtype x = embTYPE VTYPE('a) \<rbrakk> \<Longrightarrow> SemE (v :: 'a vdme) \<rhd>\<^sub>e x"
   apply (rule) back
   apply (force intro:typing defined)
   apply (force intro:defined)
 done
 
-definition EvalD :: "'a vdme \<Rightarrow> vdmv WF_BINDING \<Rightarrow> 'a" ("\<lbrakk>_\<rbrakk>\<^sub>v_") where
+definition EvalD :: "'a vdme \<Rightarrow> vdmv WF_BINDING \<Rightarrow> 'a option" ("\<lbrakk>_\<rbrakk>\<^sub>v_") where
 "\<lbrakk>v\<rbrakk>\<^sub>vb = \<langle>v\<rangle>\<^sub>v b"
 
 lemma EvalE_SemE [evale]:
